% !TeX program = lualatex
% !TeX encoding = utf-8

\documentclass[master.tex]{subfiles}
% \documentclass[11pt]{report}
% \input{./preamble.tex}

\begin{document}
\section{An axiomatic definition of the natural numbers}
We begin with a set called $\N$.
We know nothing about it yet, but we will assume these three properties to be axiomatic:
\begin{enumerate}[label=\textbf{a\arabic*)}]
    \item $1 \in \N$.\footnote{
        The standard axiomatization of $\N$ starts with $0$, but we start with $1$ to simplify our approach in constructing $\R$.
        Starting this way ultimately does not affect any of our subsequent results.
    }
    \item $n \in \N \implies (n + 1) \in \N$.
    \item If $A \subseteq \N$ is a set such that $1 \in A$ and $n \in A \implies (n + 1) \in A$, then $A = \N$.
\end{enumerate}

But what is $+$?
Remember that we know nothing about $\N$, so we cannot say right away, for example, that $1 + 1 = 2$.\footnote{
    Addition, multiplication, and other properties will be defined and proven in the exercises.
}
Instead, we generalize these axioms with an (almost) equivalent set of three other axioms.
Let $\N$ be a set containing $1$ and equipped with a function $S: \N \rightarrow \N$ such that:
\begin{enumerate}[label=\textbf{b\arabic*)}]
    \item $\Ima{(S)} = \N \setminus \set{1}$.
    \item $S$ is injective.
    \item If $A \subseteq \N$ is a set such that $1 \in A$ and $S(A) \subseteq A$, then $A = \N$.
\end{enumerate}

The formal link between these sets of axioms is the definition $S(n) := n + 1$, which we call a \emph{successor function}.
The latter set gives the standard axiomatization of the natural numbers known as the \emph{Peano axioms}.\footnote{
    Named in honor of Giuseppe Peano, 1858--1932.
}
\begin{definition}{Peano axioms}{peano-axioms}
    $\N$ is a set called the \textbf{natural numbers}, equipped with a function $S: \N \rightarrow \N$.
    \begin{enumerate}
        \item $1 \in \N$.
        \item $\Ima{(S)} = \N \setminus \set{1}$.
        \item $S$ is injective.
        \item If $A \subseteq \N$ is a set such that $1 \in A$ and $S(A) \subseteq A$, then $A = \N$.
    \end{enumerate}
\end{definition}

But do axioms \textbf{a1--3} and the Peano axioms produce the same version of $\N$?
Consider what would happen if $\N$ were a finite set.
A finite $\N$ can satisfy axioms \textbf{a1--3}, but our intuition tells us that $\N$ should be infinite.
This is further explored in the exercises.
(Note: Adding the assumption that $\N$ is infinite to axioms \textbf{a1--3} makes them equivalent to the Peano axioms).

    \subsection*{Exercises}
    \begin{enumerate}
        \item Let $\N$ be the natural numbers given by the Peano axioms. 
        Prove that $S$ is injective if and only if $\N$ is not a finite set.

        \item Prove that the fourth Peano axiom implies the principle of mathematical induction:\footnote{
            We will henceforth freely use induction as a proof technique.
        }
        \begin{quote}
            Let $P(n)$ be a proposition whose truth value depends on the value $n \in \N$.
            Suppose $P(1)$ is true and that $P(n) \implies P(n + 1)$ for all $n \geq 1$.
            Then $P(n)$ is true for all $n \in \N$.
        \end{quote}

        \item Define \emph{addition} $(+)$ in $\N$ by
        \begin{itemize}
            \item $\forall n \in \N \quad n + 1 = S(n)$, and
            \item $\forall m, n \in \N \quad n + S(m) = S(n + m)$;
        \end{itemize}
        and \emph{multiplication} $(\cdot)$ in $\N$ by
        \begin{itemize}
            \item $\forall n \in \N \quad n \cdot 1 = n$, and
            \item $\forall m, n \in \N \quad n \cdot S(m) = n \cdot m + n$.
        \end{itemize}
        Prove the following properties:
        \begin{enumerate}
            \item $n \in \N \setminus \set{1} \implies \exists! \, n' \in \N$ such that $n = S(n')$.
            \item $\forall a \in \N \quad a + 1 = 1 + a$.
            \item $+$ is associative: $\forall a, b, c \in \N \quad a + (b + c) = (a + b) + c$.
            \item $+$ is commutative: $\forall a, b \in \N \quad a + b = b + a$.
            \item $\cdot$ distributes over $+$: $\forall a, b, c \in \N \quad a \cdot (b + c) = (a \cdot b) + (a \cdot c)$.
        \end{enumerate}
    \end{enumerate}
\end{document}
